src/reflection/FStar.Reflection.Interpreter.fs
@@ -158,4 +158,7 @@ let reflection_primops : list<Cfg.primitive_step> = [
 
     mk2 "lookup_typ"            lookup_typ            E.e_env             e_string_list      (e_option E.e_sigelt)
                                 lookup_typ            NRE.e_env           NBET.e_string_list (NBET.e_option NRE.e_sigelt);
+
+    mk1 "env_open_modules"      env_open_modules      E.e_env             (e_list e_string_list)
+                                env_open_modules      NRE.e_env           (NBET.e_list NBET.e_string_list);
 ]
